@prefix dataid: <http://dataid.dbpedia.org/ns/core#> .
@prefix dcat: <http://www.w3.org/ns/dcat#> .
@prefix prov: <http://www.w3.org/ns/prov#> .
@prefix void: <http://rdfs.org/ns/void#> .
@prefix rdf: <http://www.w3.org/1999/02/22-rdf-syntax-ns#> .
@prefix rdfs: <http://www.w3.org/2000/01/rdf-schema#> .
@prefix owl: <http://www.w3.org/2002/07/owl#> .
@prefix xml: <http://www.w3.org/XML/1998/namespace> .
@prefix xsd: <http://www.w3.org/2001/XMLSchema#> .
@prefix dct: <http://purl.org/dc/terms/> .
@prefix foaf: <http://xmlns.com/foaf/0.1/> . 
@prefix skos: <http://www.w3.org/2004/02/skos/core#> .
@prefix lvont: <http://lexvo.org/ontology#> .
@prefix vann: <http://purl.org/vocab/vann/> .
@prefix odrl: <http://www.w3.org/ns/odrl/2/> .
@prefix spdx: <http://spdx.org/rdf/terms/#> .
@prefix datacite: <http://purl.org/spar/datacite/> .
@prefix lit: <http://www.essepuntato.it/2010/06/literalreification/> .

@base <http://dataid.dbpedia.org/ns/core#> .

dataid:
    a owl:Ontology ;
    owl:imports dcat:, prov: ; #, foaf:, datacite: ;
    vann:preferredNamespaceUri "http://dataid.dbpedia.org/ns/core#" ;
    vann:preferredNamespacePrefix "dataid" ;
    owl:versionInfo "2.0.0" ; 
    dct:modified "2016-12-07" ;
    rdfs:comment """The DataID core ontology is the central part of the DataID multi-layered metadata system. 
Its goal is to extensively describes datasets and their different manifestations in a uniform way, 
as well as relations with agents such as persons or organisations, in regard to their rights and responsibilities. 
Established vocabularies such as DCAT, VoID, Prov-O are used for maximum compatibility.
We introduced a multilayer concept of supporting ontologies extending DataID core to fit different 
use case scenarios (for Linked Data, providing statistical data about datasets etc.).
By describing datasets including content, authors, licenses and provenance via RDF, thereby making data 
accessible to others, is the basic idea of Linked Open Data and is your contribution to a 
universal data give and take. You can create your own DataID files for any type of data at http://dataid.dbpedia.org.
Validating and delivering metadata files in a uniform way, as well as providing the ability to query for datasets, 
are main objectives of the DBpedia/DataID project."""@en ;
    rdfs:label "DataID"@en ;
    foaf:depiction 	<https://raw.githubusercontent.com/dbpedia/DataId-Ontology/master/DataIdOntology.png> ;
    foaf:homepage 	<http://wiki.dbpedia.org/projects/dbpedia-dataid> ;
    foaf:page 	<https://github.com/dbpedia/DataId-Ontology> ;
	dct:license <http://purl.org/NET/rdflicense/cc-by4.0> ;
	dct:creator <http://wiki.dbpedia.org/Association/Persons/Freudenberg> ;
	dct:contributor <http://aksw.org/MartinBruemmer.html> .
    
<http://wiki.dbpedia.org/Association/Persons/Freudenberg>
    a                        dataid:Agent ;
    foaf:mbox                "freudenberg@informatik.uni-leipzig.de" ;
    foaf:homepage			<http://wiki.dbpedia.org/Association/Persons/Freudenberg> ;
    foaf:homepage			<http://aksw.org/MarkusFreudenberg.html> ;
    foaf:name                "Markus Freudenberg" .
    
########### classes ##########
    
dataid:DataId
	a owl:Class ;
    rdfs:isDefinedBy <http://dataid.dbpedia.org/ns/core#> ;
    rdfs:label "DataId"@en ;
	rdfs:comment """The dataid:DataId class is the most generic entity in a DataID graph about one or more datasets. 
	As a subclass of dcat:CatalogRecord / void:DatasetDescription it describes not a dataset itself but provides metadata about 
	its entry in a dcat:Catalog and/or its relations to repositories or other data collections."""@en ;
	rdfs:subClassOf void:DatasetDescription, dcat:CatalogRecord, prov:Entity,
		[
	        a owl:Restriction ;
	        owl:allValuesFrom dataid:Dataset ;
	        owl:onProperty foaf:primaryTopic
	    ],[
	        a owl:Restriction ;
	        owl:allValuesFrom dataid:DataId ;
	        owl:onProperty dataid:nextVersion
	    ],[
	        a owl:Restriction ;
	        owl:allValuesFrom dataid:DataId ;
	        owl:onProperty dataid:previousVersion
	    ],[
	        a owl:Restriction ;
	        owl:allValuesFrom dataid:DataId ;
	        owl:onProperty dataid:latestVersion
	    ],[
	        a owl:Restriction ;
	        owl:allValuesFrom odrl:Policy;
	        owl:onProperty dct:license
	    ],[
	        a owl:Restriction ;
	        owl:allValuesFrom lvont:Language ;
	        owl:onProperty dct:language
	    ],[
	        a owl:Restriction ;
	        owl:allValuesFrom dataid:SimpleStatement ;
	        owl:onProperty dct:rights
	    ].	    

dataid:Dataset
    a owl:Class ;
    rdfs:isDefinedBy <http://dataid.dbpedia.org/ns/core#> ;
    rdfs:label "Dataset"@en ;
    rdfs:comment """A collection of data, available for access in one or more formats. 
    Dataset resources describe the concept of the dataset, not its manifestation (the data itself), which can be acquired 
    as a Distribution. Datasets are prov:Entities and can be generated by prov:Activities."""@en ;
    rdfs:subClassOf void:Dataset, dcat:Dataset, prov:Entity,
    	[
	        a owl:Restriction ;
	        owl:allValuesFrom dataid:DataId ;
	        owl:onProperty foaf:isPrimaryTopicOf
	    ],[
	        a owl:Restriction ;
	        owl:allValuesFrom dataid:Dataset ;
	        owl:onProperty dataid:nextVersion
	    ],[
	        a owl:Restriction ;
	        owl:allValuesFrom dataid:Dataset ;
	        owl:onProperty dataid:previousVersion
	    ],[
	        a owl:Restriction ;
	        owl:allValuesFrom dataid:Dataset ;
	        owl:onProperty dataid:latestVersion
	    ],[
	        a owl:Restriction ;
	        owl:allValuesFrom odrl:Policy ;
	        owl:onProperty dct:license
	    ],[
	        a owl:Restriction ;
	        owl:allValuesFrom lvont:Language ;
	        owl:onProperty dct:language
	    ],[ 
			a owl:Restriction ;
			owl:onProperty dct:isPartOf ;
		 	owl:allValuesFrom dataid:Dataset
	 	],[ 
			a owl:Restriction ;
			owl:onProperty void:subset ;
		 	owl:allValuesFrom dataid:Dataset
	 	],[
	        a owl:Restriction ;
	        owl:onProperty dcat:distribution ;
	        owl:allValuesFrom dataid:Distribution 
	    ],[
	        a owl:Restriction ;
	        owl:allValuesFrom <http://www.w3.org/2006/time#Interval> ;
	        owl:onProperty dct:temporal
	    ],[
	        a owl:Restriction ;
	        owl:allValuesFrom <http://www.geonames.org/ontology#Feature> ;
	        owl:onProperty dct:spatial
	    ],[
	        a owl:Restriction ;
	        owl:allValuesFrom dataid:SimpleStatement ;
	        owl:onProperty dct:rights
	    ].
	    
dataid:Superset
    a owl:Class ;
    rdfs:isDefinedBy <http://dataid.dbpedia.org/ns/core#> ;
    rdfs:label "Superset"@en ;
    rdfs:comment """This dedicated version of a dataid:Dataset has exacly one purpose: to point out all its Sub-Datsets with void:subset. 
    A dataid:Superset has no data itself and is therefore prohibited to point out Distributions with dcat:distribution. 
    It can be used in a dataset hierarchy (e.g. as a root dataset), or as a container for other datasets."""@en ;
    rdfs:subClassOf dataid:Dataset,
    [  
    	# owl:maxCardinality 0 or 1 does not break OWL 2 RL
        a owl:Restriction ;
        owl:maxCardinality "0"^^xsd:nonNegativeInteger ;
        owl:onProperty dcat:distribution
    ].

dataid:Distribution
    a owl:Class ;
    rdfs:isDefinedBy <http://dataid.dbpedia.org/ns/core#> ;
    rdfs:comment """Distributions describe the technical details of a single manifestation of the pertaining Dataset 
    (for example; its data format/serialisation or a ServiceEndpoint including the procedure required to access the data)."""@en ;
    rdfs:label "Distribution"@en ;
    rdfs:subClassOf dcat:Distribution, prov:Entity,
    	[
	        a owl:Restriction ;
	        owl:allValuesFrom dataid:Distribution ;
	        owl:onProperty dataid:nextVersion
	    ],[
	        a owl:Restriction ;
	        owl:allValuesFrom dataid:Distribution ;
	        owl:onProperty dataid:previousVersion
	    ],[
	        a owl:Restriction ;
	        owl:allValuesFrom dataid:Distribution ;
	        owl:onProperty dataid:latestVersion
	    ],[
	        a owl:Restriction ;
	        owl:allValuesFrom odrl:Policy ;
	        owl:onProperty dct:license
	    ],[
	        a owl:Restriction ;
	        owl:allValuesFrom lvont:Language ;
	        owl:onProperty dct:language
	    ],[
	        a owl:Restriction ;
	        owl:allValuesFrom dataid:SimpleStatement ;
	        owl:onProperty dct:rights
	    ].

dataid:ServiceEndpoint
    a owl:Class ;
    rdfs:isDefinedBy <http://dataid.dbpedia.org/ns/core#> ;
    rdfs:comment "A specific Distribution, which is accessible via an access URL and provides data as a web service in a certain format."@en ;
    rdfs:label "Service Endpoint"@en ;
    rdfs:subClassOf dataid:Distribution. 

dataid:SingleFile
    a owl:Class ;
    rdfs:isDefinedBy <http://dataid.dbpedia.org/ns/core#> ;
    rdfs:comment "A single data dump file representing the whole Dataset, in a certain format/serialisation."@en ;
    rdfs:label "Single File"@en ;
    rdfs:subClassOf dataid:Distribution.

dataid:Directory
    a owl:Class ;
    rdfs:isDefinedBy <http://dataid.dbpedia.org/ns/core#> ;
    rdfs:comment "A dedicated file system directory holding (multiple) files of the same Dataset, which, when put together, make up the whole Dataset."@en ;
    rdfs:label "Directory"@en ;
    rdfs:subClassOf dataid:Distribution.

dataid:FileCollection
    a owl:Class ;
    rdfs:isDefinedBy <http://dataid.dbpedia.org/ns/core#> ;
    rdfs:comment "Multiple files constituting one (complete) Dataset (files in different directories or servers are allowed, as opposed to Directory)."@en ;
    rdfs:label "File Collection"@en ;
    rdfs:subClassOf dataid:Distribution.
    
dataid:DatasetRelationship
	a owl:Class;
	rdfs:isDefinedBy <http://dataid.dbpedia.org/ns/core#> ;
    rdfs:comment "Portrays a generic relation between two or more datasets."@en ;
    rdfs:label "Dataset Relationship"@en ;
    rdfs:subClassOf prov:EntityInfluence.
    
dataid:DatasetRelationRole
	a owl:Class;
	rdfs:isDefinedBy <http://dataid.dbpedia.org/ns/core#> ;
    rdfs:comment "Provides the role of a dataid:DatasetRelationship (e.g. Linkset, Source, Derivat, Similarity etc.)."@en ;
    rdfs:label "Dataset Relation Role"@en ;
    rdfs:subClassOf prov:Role.
    
dataid:Agent
    a owl:Class ;
    rdfs:isDefinedBy <http://dataid.dbpedia.org/ns/core#> ;
    rdfs:comment "Agents are real or legal persons, groups of persons, programs, organisations etc."@en ;
    rdfs:label "Agent"@en ;
    rdfs:subClassOf prov:Agent, foaf:Agent, dct:Agent.

dataid:Authorization
	a owl:Class ;
    rdfs:isDefinedBy <http://dataid.dbpedia.org/ns/core#> ;
    rdfs:label "Authorization"@en ;
	rdfs:comment """This concept is a mediator between a set of Entities (or scope) defined by the property dataid:authorizedFor, a set of AgentRoles 
  defining rights and responsibilities (dataid:authorityAgentRole) and Agents (dataid:associatedAgent), fulfilling the AgentRoles, 
  in regard to the collection of Entities. This subclass of prov:Attribution qualifies the relation prov:wasAttributedTo between prov:Entity 
  and prov:Agent with the AgentRoles and AuthorizedActions of the DataID-domain."""@en ;
	rdfs:subClassOf prov:Attribution .

dataid:AgentRole
	a owl:Class ;
    rdfs:isDefinedBy <http://dataid.dbpedia.org/ns/core#> ;
    rdfs:label "Agent Role"@en ;
	rdfs:comment """AgentRoles are defined by a set of rights and responsibilities (see AuthorizedAction) an Agent, assigned with this Role, has to address or can execute."""@en ;
	rdfs:subClassOf prov:Role, skos:Concept .

dataid:AuthorizedAction
	a owl:Class ;
	rdfs:subClassOf skos:Concept ;
    rdfs:isDefinedBy <http://dataid.dbpedia.org/ns/core#> ;
    rdfs:label "Authorized Action"@en ;
    rdfs:comment """AuthorizedActions may be comprised either of activities an Agent can execute in regard to a collection of Entities (dataid:EntitledAction), 
    or of responsibilities an Agent should act upon (dataid:ResponsibleAction) (e.g. make certain decisions if necessary or act upon certain events)."""@en .

dataid:ResponsibleAction
	a owl:Class ;
    rdfs:isDefinedBy <http://dataid.dbpedia.org/ns/core#> ;
    rdfs:label "Responsible Action"@en ;
	rdfs:comment """AgentRoles provide rights as well as responsibilities an agent has to attend to in order to fulfil this Role. 
  ResponsibleActions should describe actions pertaining to responsibilities an agent is supposed to do when holding a specific AgentRole."""@en ;
	rdfs:subClassOf dataid:AuthorizedAction ;
	owl:disjointWith dataid:EntitledAction .

dataid:EntitledAction
	a owl:Class ;
    rdfs:isDefinedBy <http://dataid.dbpedia.org/ns/core#> ;
    rdfs:label "Entitled Action"@en ;
	rdfs:comment """EntitledActions describe actions an Agent is allowed to perform when holding a certain AgentRole. These Actions may address restricted matters like access, modification rights and others."""@en ;
	rdfs:subClassOf dataid:AuthorizedAction ;
	owl:disjointWith dataid:ResponsibleAction .
	
dataid:SimpleStatement
	a owl:Class;
	rdfs:isDefinedBy <http://dataid.dbpedia.org/ns/core#> ;
	rdfs:label "Simple Statement"@en ;
	rdfs:comment """A SimpleStatement is intended as a tool for conveying a statement, definition or point of view about a certain topic. Using either a simple literal (using dataid:literal) to provide a quotation or by a referencing a web resource providing or representing the statement in any given medium (picture, text, video etc.). This class implements several classes of Dublin Core which is not further specified within DC."""@en ;
	rdfs:subClassOf prov:Entity, dct:ProvenanceStatement, dct:RightsStatement, dct:Standard, lit:Literal,
	[
        a owl:Restriction ;
        owl:allValuesFrom foaf:Document ;
        owl:onProperty dct:references
    ].

dataid:Identifier
	a owl:Class ;
	rdfs:isDefinedBy <http://dataid.dbpedia.org/ns/core#> ;
	rdfs:label "Identifier"@en ;
	rdfs:comment """Uniquely identifies any resource, given an identifier as literal (see dataid:literal) and a corresponding identifier scheme (e.g. a aid/pid scheme such as ORCID, ResearcherID etc. pointed out via datacite:usesIdentifierScheme). Optionally it can point out a reference document on the web (about this Identifier) using dct:references."""@en ;
	rdfs:subClassOf datacite:Identifier, lit:Literal,
	[
        a owl:Restriction ;
        owl:allValuesFrom foaf:Document ;
        owl:onProperty dct:references
    ].
	    
dataid:MediaType
	a owl:Class;
	rdfs:isDefinedBy <http://dataid.dbpedia.org/ns/core#> ;
	rdfs:label "Media Type"@en ;
	rdfs:comment """Extends the dct:MediaTypeOrExtend class of Dublin Core, providing the IANA media type description (or mime type) and common file extensions used. 
  A pointer to an inner media (dataid:innerMediaType) can describe (multiple) layers of compressions and all internal media types."""@en ;
	rdfs:subClassOf dct:MediaType.
		
########## properties #########
		
dataid:accessProcedure
	a owl:ObjectProperty ;
	rdfs:isDefinedBy <http://dataid.dbpedia.org/ns/core#> ;
	rdfs:comment "Describes the steps which have to be taken to gain access to the described data at the location of a Distribution (e.g. register an account to gain dct:accessRights)."@en ;
    rdfs:domain dataid:Distribution ;
    rdfs:label "access procedure"@en ;
    rdfs:range dataid:SimpleStatement .

dataid:isDistributionOf
	a	owl:ObjectProperty ;
	rdfs:isDefinedBy <http://dataid.dbpedia.org/ns/core#> ;
	rdfs:label "is distribution of"@en ;
	rdfs:comment "Inverse property of dcat:distribution, linking a Distribution to a Dataset."@en ;
	owl:inverseOf	dcat:distribution;
	rdfs:domain		dataid:Distribution;
	rdfs:range		dataid:Dataset.

dataid:inCatalog
	a	owl:ObjectProperty ;
	rdfs:isDefinedBy <http://dataid.dbpedia.org/ns/core#> ;
	rdfs:label "in catalog"@en ;
	rdfs:comment "The inverse property of dcat:record, pointing back to the dcat:Catalog in which this DataId is recorded."@en ;
	owl:inverseOf	dcat:record;
	rdfs:domain		dataid:DataId;
	rdfs:range		dcat:Catalog.
	
dataid:uncompressedByteSize
	a	owl:DatatypeProperty ;
	rdfs:subPropertyOf dcat:byteSize ;
	rdfs:isDefinedBy <http://dataid.dbpedia.org/ns/core#> ;
	rdfs:label "uncompressed byte size"@en ;
	rdfs:comment "Records the byte size of the uncompressed content of an archive file."@en ;
	rdfs:domain		dataid:Distribution ;
    rdfs:range      xsd:integer.

dataid:qualifiedDatasetRelation
	a	owl:ObjectProperty, owl:InverseFunctionalProperty;
	rdfs:subPropertyOf prov:qualifiedInfluence;
	rdfs:isDefinedBy <http://dataid.dbpedia.org/ns/core#> ;
	rdfs:label "relation of"@en ;
	rdfs:comment "Qualifies the dataid:relatedDatset property with a DatasetRelationship."@en ;
	rdfs:domain		dataid:Dataset;
	rdfs:range		dataid:DatasetRelationship.
	
dataid:qualifiedRelationOf
	a	owl:ObjectProperty, owl:FunctionalProperty ;
	owl:inverseOf	dataid:qualifiedDatasetRelation;
	rdfs:isDefinedBy <http://dataid.dbpedia.org/ns/core#> ;
	rdfs:label "qualified relation of"@en ;
	rdfs:comment "Inverse property of dataid:qualifiedDatasetRelation, pointing out a dataset which has related datasets referred to via dataid:dataid:qualifiedRelationTo."@en .
		
dataid:qualifiedRelationTo
	a	owl:ObjectProperty ;
	rdfs:subPropertyOf prov:entity;
	rdfs:isDefinedBy <http://dataid.dbpedia.org/ns/core#> ;
	rdfs:label "qualified relation to"@en ;
	rdfs:comment "Pointing out datasets which are somehow related to the dataset referred to via dataid:dataid:qualifiedRelationOf."@en ;
	rdfs:domain		dataid:DatasetRelationship;
	rdfs:range		dataid:Dataset.
	
dataid:datasetRelationRole
	a	owl:ObjectProperty ;
	rdfs:subPropertyOf prov:hadRole;
	rdfs:isDefinedBy <http://dataid.dbpedia.org/ns/core#> ;
	rdfs:label "dataset relation role"@en ;
	rdfs:comment "The role which qualifies a dataid:DatasetRelationship. It specifies which relationship datasets (pointed out with dataid:qualifiedRelationTo) have in regard to the dataset referred to with dataid:qualifiedRelationOf (e.g. source datasets when dataid:SourceRole is in place)."@en ;
	rdfs:domain		dataid:DatasetRelationship;
	rdfs:range		dataid:DatasetRelationRole.
	
dataid:relatedDataset
    a owl:ObjectProperty, owl:SymmetricProperty;
    rdfs:subPropertyOf dct:relation, prov:wasInfluencedBy ;
    rdfs:isDefinedBy <http://dataid.dbpedia.org/ns/core#> ;
    rdfs:comment 	"Points to other Datasets containing related data. Can be qualified with dataid:DatasetRelationship. (note: while this property is symmetric, its qualification is not)"@en ;
    rdfs:domain 	dataid:Dataset ;
    rdfs:label 		"related dataset"@en ;
    rdfs:range  	dataid:Dataset ;
    owl:propertyChainAxiom (
	   dataid:qualifiedDatasetRelation
	   dataid:qualifiedRelationTo
	).

dataid:preview
    a owl:ObjectProperty ;
    rdfs:isDefinedBy <http://dataid.dbpedia.org/ns/core#> ;
    rdfs:comment 	"Provides the URL of a short preview of the data provided by a Distribution, helpful when conveying type and format of the data provided as an example."@en ;
    rdfs:domain 	dataid:Distribution ;
    rdfs:label 		"preview"@en ;
    rdfs:range  	foaf:Document .
    
dataid:associatedAgent
    a owl:ObjectProperty ;
    rdfs:subPropertyOf prov:wasAttributedTo ;
    rdfs:isDefinedBy <http://dataid.dbpedia.org/ns/core#> ;
    rdfs:comment "An Agent which is generally connected to the Dataset. Their exact function in regard to the Entity has to be specified by the qualification of an Authorization."@en ;
    rdfs:domain prov:Entity ;
    rdfs:label "associated agent"@en ;
    rdfs:range dataid:Agent ;
    owl:propertyChainAxiom (
	   dataid:underAuthorization
	   dataid:authorizedAgent
	) .

dataid:softwareRequirement
    a owl:ObjectProperty ;
    rdfs:isDefinedBy <http://dataid.dbpedia.org/ns/core#> ;
    rdfs:comment "Software needed to access the data provided via this Distribution or otherwise relevant for consuming the data."@en ;
    rdfs:domain dataid:Distribution ;
    rdfs:label "software requirement"@en ;
    rdfs:range dataid:SimpleStatement .
    
dataid:checksum
    a owl:ObjectProperty ;
    rdfs:isDefinedBy <http://dataid.dbpedia.org/ns/core#> ;
    rdfs:comment """The checksum value allows the contents of a file to be authenticated since it shifts even with small changes to the file."""@en ;
    rdfs:domain dataid:Distribution	;
    rdfs:label "checksum"@en ;
    rdfs:range spdx:Checksum .

dataid:previousVersion
    a owl:ObjectProperty ;
    rdfs:subPropertyOf prov:wasDerivedFrom;
    rdfs:isDefinedBy <http://dataid.dbpedia.org/ns/core#> ;
    rdfs:comment "Previous version of a DataId/Dataset/Distribution."@en ;
    rdfs:domain prov:Entity ;
    rdfs:label "previous version"@en ;
    rdfs:range prov:Entity .

dataid:nextVersion
    a owl:ObjectProperty ;
    rdfs:isDefinedBy <http://dataid.dbpedia.org/ns/core#> ;
   	owl:inverseOf dataid:previousVersion ;
    rdfs:comment "Next version of a DataId/Dataset/Distribution."@en ;
    rdfs:label "next version"@en .
    
dataid:latestVersion
    a owl:ObjectProperty ;
    rdfs:isDefinedBy <http://dataid.dbpedia.org/ns/core#> ;
    rdfs:comment "Latest version of a DataId/Dataset/Distribution."@en ;
    rdfs:domain prov:Entity ;
    rdfs:label "latest version"@en ;
    rdfs:range prov:Entity .

dataid:innerMediaType 
	a owl:ObjectProperty, owl:FunctionalProperty ;
	rdfs:subPropertyOf dcat:mediaType;
	rdfs:isDefinedBy <http://dataid.dbpedia.org/ns/core#> ;
    rdfs:comment "Points out the MediaType of the (compressed) file inside another file (relevant for archive files)."@en ;
    rdfs:domain dataid:MediaType ;
    rdfs:label "inner media type"@en ;
    rdfs:range dataid:MediaType .
    
dataid:typeTemplate
	a owl:DatatypeProperty, owl:FunctionalProperty ;
	rdfs:isDefinedBy <http://dataid.dbpedia.org/ns/core#> ;
	rdfs:comment "The template (or mime type string) of a MediaType."@en ;
    rdfs:domain dataid:MediaType ;
    rdfs:label "media type template"@en ;
    rdfs:range rdfs:Literal .
    
dataid:typeReference
	a owl:ObjectProperty;
	rdfs:subPropertyOf	foaf:page ;
	rdfs:isDefinedBy <http://dataid.dbpedia.org/ns/core#> ;
	rdfs:comment "Refers to a standard document of the MediaType described."@en ;
    rdfs:domain dataid:MediaType ;
    rdfs:label "media type reference"@en .
    
dataid:typeExtension
	a owl:DatatypeProperty;
	rdfs:isDefinedBy <http://dataid.dbpedia.org/ns/core#> ;
	rdfs:comment "Lists file extensions commonly used with this MediaType."@en ;
    rdfs:domain dataid:MediaType ;
    rdfs:label "media type file extension"@en ;
    rdfs:range rdfs:Literal .
	    
dataid:typeName
	a owl:DatatypeProperty;
	rdfs:isDefinedBy <http://dataid.dbpedia.org/ns/core#> ;
	rdfs:comment "Names the MediaType described."@en ;
    rdfs:domain dataid:MediaType ;
    rdfs:label "media type name"@en ;
    rdfs:range rdfs:Literal .
    
dataid:literal
	a owl:DatatypeProperty ;
	rdfs:subPropertyOf lit:hasLiteralValue;
	rdfs:isDefinedBy <http://dataid.dbpedia.org/ns/core#> ;
    rdfs:comment 	"An actual textual statement or literal (string)."@en ;
    rdfs:label "statement"@en ;
    rdfs:range rdfs:Literal.

dataid:identifier
    a owl:ObjectProperty, owl:InverseFunctionalProperty ;
    rdfs:subPropertyOf datacite:hasIdentifier, foaf:isPrimaryTopicOf ;
    rdfs:isDefinedBy <http://dataid.dbpedia.org/ns/core#> ;
    rdfs:comment "A unique identifier for an Agent or Entity (for other, non DataID related identifiers)."@en ;
    rdfs:label "identifier"@en ;
    rdfs:range datacite:Identifier .

dataid:authorizedAgent
   	a owl:ObjectProperty ;
    rdfs:subPropertyOf prov:agent ;
   	rdfs:isDefinedBy <http://dataid.dbpedia.org/ns/core#> ;
    rdfs:comment "Points out an Agent which holds the rights granted by an Authorization (e.g. to modify the metadata of a Dataset)."@en ;
    rdfs:domain prov:AgentInfluence ;
    rdfs:label "authorized agent"@en ;
    rdfs:range dataid:Agent .

dataid:hasAuthorization
   	a owl:ObjectProperty ;
   	owl:inverseOf dataid:authorizedAgent ;
   	rdfs:isDefinedBy <http://dataid.dbpedia.org/ns/core#> ;
    rdfs:comment "Provides an Agent with the Authorization for a given scope of Entities (e.g. Dataset, Distribution etc.), granting rights to execute certain AuthorizedActions."@en ;
    rdfs:label "has authorization"@en .
    
dataid:authorityAgentRole
   	a owl:ObjectProperty ;
    rdfs:subPropertyOf prov:hadRole ;
    rdfs:isDefinedBy <http://dataid.dbpedia.org/ns/core#> ;
    rdfs:comment "Assigns an AgentRole for an Authorization to an Agent, thereby allowing for certain AuthorizedActions this Agent can execute on the Entities defined by the scope of the Authorization."@en ;
    rdfs:domain prov:AgentInfluence ;
    rdfs:label "authority agent role"@en ;
    rdfs:range dataid:AgentRole .

dataid:allowsFor
   	a owl:ObjectProperty ;
    rdfs:isDefinedBy <http://dataid.dbpedia.org/ns/core#> ;
    rdfs:comment "An AgentRole allows an Agent to execute certain AuthorizedActions."@en ;
    rdfs:domain dataid:AgentRole ;
    rdfs:label "allows for"@en ;
    rdfs:range dataid:AuthorizedAction .

dataid:authorizedAction
   	a owl:ObjectProperty ;
    rdfs:isDefinedBy <http://dataid.dbpedia.org/ns/core#> ;
    rdfs:comment "Points out AuthorizedActions Agents are allowed to execute under a given Authorization (and its chosen AgentRoles)."@en ;
    rdfs:domain prov:AgentInfluence ;
    rdfs:label "authorized action"@en ;
    rdfs:range dataid:AuthorizedAction ;
    owl:propertyChainAxiom (
	   dataid:authorityAgentRole
	   dataid:allowsFor
	) .
	
dataid:identifierScheme
    a owl:ObjectProperty ;
    rdfs:isDefinedBy <http://dataid.dbpedia.org/ns/core#> ;
    rdfs:comment "Points out which scheme of identifiers is used to uniquely identify resources inside a Dataset."@en ;
    rdfs:label "identifier scheme"@en ;
    rdfs:domain dataid:Dataset ;
    rdfs:range datacite:IdentifierScheme .

dataid:usefulness 
	a owl:ObjectProperty ;
	rdfs:isDefinedBy <http://dataid.dbpedia.org/ns/dmp#> ;
	rdfs:label "usefulness"@en ;
	rdfs:comment "Description of to whom the Dataset could be useful, and whether it underpins a scientific publication."@en ;
	rdfs:domain dataid:Dataset ;
	rdfs:range dataid:SimpleStatement .

dataid:similarData 
	a owl:ObjectProperty ;
	rdfs:isDefinedBy <http://dataid.dbpedia.org/ns/dmp#> ;
   	rdfs:label "similar data"@en ;
   	rdfs:comment "Information on the existence (or absence) of similar data (see also dataid:similarDataset)."@en ;
   	rdfs:domain dataid:Dataset ;
   	rdfs:range dataid:SimpleStatement .

dataid:reuseAndIntegration 
	a owl:ObjectProperty ;
	rdfs:isDefinedBy <http://dataid.dbpedia.org/ns/dmp#> ;
	rdfs:label "reuse and integration"@en ;
	rdfs:comment "Information on the possibilities for integration and reuse of the Dataset."@en ;
	rdfs:domain dataid:Dataset ;
	rdfs:range dataid:SimpleStatement .

dataid:growth 
	a owl:ObjectProperty ;
	rdfs:isDefinedBy <http://dataid.dbpedia.org/ns/dmp#> ;
	rdfs:label "growth"@en ;
	rdfs:comment "Indication of what size the approximated end volume of the Dataset is."@en ;
	rdfs:domain dataid:Dataset ;
	rdfs:range dataid:SimpleStatement .

dataid:openness 
	a owl:ObjectProperty ;
	rdfs:isDefinedBy <http://dataid.dbpedia.org/ns/dmp#> ;
	rdfs:label "openness"@en ;
	rdfs:comment """General description of how data will be shared. For example embargo periods (if any), outlines of technical mechanisms for dissemination or a definition of whether access will be widely open or restricted to specific groups. In case the Dataset cannot be shared, the reasons for this should be mentioned (e.g. ethical, rules of personal data, intellectual property, commercial, privacy-related, security-related)."""@en ;
	rdfs:domain dataid:Dataset ;
	rdfs:range dataid:SimpleStatement .

dataid:dataDescription
	a owl:ObjectProperty ;
	rdfs:isDefinedBy <http://dataid.dbpedia.org/ns/dmp#> ;
	rdfs:label "data description"@en ;
	rdfs:comment "Provides a detailed description of the data represented by this Dataset."@en ;
	rdfs:domain dataid:Dataset ;
	rdfs:range dataid:SimpleStatement .

dataid:validFrom
    a owl:DatatypeProperty, owl:FunctionalProperty ;
    rdfs:isDefinedBy <http://dataid.dbpedia.org/ns/core#> ;
    rdfs:comment 	"The influence an Agent has over an Entity is valid from (inclusive) a certain point in time."@en ;
    rdfs:domain 	prov:AgentInfluence ;
    rdfs:label 		"valid from"@en ;
    rdfs:range  	xsd:dateTime .
    
dataid:validUntil
    a owl:DatatypeProperty, owl:FunctionalProperty ;
    rdfs:isDefinedBy <http://dataid.dbpedia.org/ns/core#> ;
    rdfs:comment 	"The influence an Agent has over an Entity is valid until (exclusive) a certain point in time."@en ;
    rdfs:domain 	prov:AgentInfluence ;
    rdfs:label 		"valid until"@en ;
    rdfs:range  	xsd:dateTime .

dataid:isInheritable
	a	owl:DatatypeProperty, owl:FunctionalProperty ;
	rdfs:isDefinedBy <http://dataid.dbpedia.org/ns/core#> ;
	rdfs:label "is inheritable"@en ;
	rdfs:comment "Indicates whether this Authorization will be valid after an update to the DataID or a scope element."@en ;
	rdfs:domain		dataid:Authorization ;
    rdfs:range      xsd:boolean.

#The follwing properties are used to defines the scope of an Authorization over multiple entities.	
dataid:authorizationScope
	a owl:ObjectProperty, owl:TransitiveProperty;
    rdfs:isDefinedBy <http://dataid.dbpedia.org/ns/core#> ;
    rdfs:comment """This property defines the scope of an Authorization. An Agent has the right to execute AuthorizedActions for all Entities of this scope.
    Together with its sub-properties (dataid:authorizedFor, dataid:authorizationChainX), it defines how the scope of an Authorization is extended to other Entities. 
    Since this property can be inferred by its sub-properties it shall not be instantiated in a DataID document."""@en ;
    rdfs:label "authorization scope"@en ;
    rdfs:range  prov:Entity .
    
dataid:authorizedFor
	a owl:ObjectProperty ;
	rdfs:subPropertyOf dataid:authorizationScope;
    rdfs:isDefinedBy <http://dataid.dbpedia.org/ns/core#> ;
    rdfs:comment """Points out the Entities which are under the direct influence of an Authorization. 
    An Agent has the right to execute AuthorizedActions (as defined by the pertaining AgentRole) for these Entities.
    This property shall be used to point out the initial entities for which an Authorization is valid. Inference via 
    authorizationChain properties may extend the scope of this Authorization further over multiple Entities along the hirarical structure of a DataID."""@en ;
    rdfs:label "authorized for"@en ;
    rdfs:domain dataid:Authorization ;
    rdfs:range  prov:Entity .
	
dataid:underAuthorization
    a owl:ObjectProperty ;
    rdfs:subPropertyOf prov:qualifiedAttribution ;
    rdfs:isDefinedBy <http://dataid.dbpedia.org/ns/core#> ;
    rdfs:comment "Points out an Authorization which grants some degree of authority over this resource (inverse property of dataid:authorizationScope)."@en ;
    rdfs:label "under authorization"@en ;
    rdfs:domain	prov:Entity ;
    rdfs:range dataid:Authorization .

dataid:needsSpecialAuthorization
    a owl:ObjectProperty ;
    rdfs:subPropertyOf dataid:underAuthorization ;
    rdfs:isDefinedBy <http://dataid.dbpedia.org/ns/core#> ;
    rdfs:comment "Points out an Authorization which grants some degree of authority over this resource to the exclusion of other Authorizations which are not referred with this property."@en ;
    rdfs:label "needs special authorization"@en ;
    rdfs:domain	prov:Entity ;
    rdfs:range dataid:Authorization .

                
#The following 9 properties are necessary to 'simulate' making foaf:primaryTopic, void:subset and dcat:distribution a rdfs:subPropertyOf dataid:authorizationScope, as not to hijack the pertaining ontologies.    
dataid:authorizationChain1
	a owl:ObjectProperty ;
	rdfs:subPropertyOf	dataid:authorizationScope ;
    rdfs:isDefinedBy <http://dataid.dbpedia.org/ns/core#> ;
	rdfs:label "Authorization Chain 1 property"@en;
    rdfs:comment "With the help of this property we can extend the reach dataid:authorizationScope over multiple instances of dataid:Dataset and dataid:Distribution."@en ;
    rdfs:range  prov:Entity ;
    owl:propertyChainAxiom (
	   foaf:primaryTopic
	   dcat:distribution
	) .
	
dataid:authorizationChain2
	a owl:ObjectProperty ;
	rdfs:subPropertyOf	dataid:authorizationScope ;
    rdfs:isDefinedBy <http://dataid.dbpedia.org/ns/core#> ;
	rdfs:label "Authorization Chain 2 property"@en;
    rdfs:comment "With the help of this property we can extend the reach dataid:authorizationScope over multiple instances of dataid:Dataset and dataid:Distribution."@en ;
    rdfs:range  prov:Entity ;
    owl:propertyChainAxiom (
	   foaf:primaryTopic
	   void:subset
	) .
	
dataid:authorizationChain3
	a owl:ObjectProperty ;
	rdfs:subPropertyOf	dataid:authorizationScope ;
    rdfs:isDefinedBy <http://dataid.dbpedia.org/ns/core#> ;
	rdfs:label "Authorization Chain 3 property"@en;
    rdfs:comment "With the help of this property we can extend the reach dataid:authorizationScope over multiple instances of dataid:Dataset and dataid:Distribution."@en ;
    rdfs:range  prov:Entity ;
    owl:propertyChainAxiom (
	   void:subset
	   dcat:distribution
	) .
	
dataid:authorizationChain4
	a owl:ObjectProperty ;
	rdfs:subPropertyOf	dataid:authorizationScope ;
    rdfs:isDefinedBy <http://dataid.dbpedia.org/ns/core#> ;
	rdfs:label "Authorization Chain 4 property"@en;
    rdfs:comment "With the help of this property we can extend the reach dataid:authorizationScope over multiple instances of dataid:Dataset and dataid:Distribution."@en ;
    rdfs:range  prov:Entity ;
    owl:propertyChainAxiom (
	   void:subset
	   void:subset
	) .
	
dataid:authorizationChain5
	a owl:ObjectProperty ;
	rdfs:subPropertyOf	dataid:authorizationScope ;
    rdfs:isDefinedBy <http://dataid.dbpedia.org/ns/core#> ;
	rdfs:label "Authorization Chain 5 property"@en;
    rdfs:comment "With the help of this property we can extend the reach dataid:authorizationScope over multiple instances of dataid:Dataset and dataid:Distribution."@en ;
    rdfs:range  prov:Entity ;
    owl:propertyChainAxiom (
	   void:subset
	   void:subset
	   dcat:distribution
	) .
	
dataid:authorizationChain6
	a owl:ObjectProperty ;
	rdfs:subPropertyOf	dataid:authorizationScope ;
    rdfs:isDefinedBy <http://dataid.dbpedia.org/ns/core#> ;
	rdfs:label "Authorization Chain 6 property"@en;
    rdfs:comment "With the help of this property we can extend the reach dataid:authorizationScope over multiple instances of dataid:Dataset and dataid:Distribution."@en ;
    rdfs:range  prov:Entity ;
    owl:propertyChainAxiom (
	   foaf:primaryTopic
	   void:subset
	   dcat:distribution
	) .
		
dataid:authorizationChain7
	a owl:ObjectProperty ;
	rdfs:subPropertyOf	dataid:authorizationScope ;
    rdfs:isDefinedBy <http://dataid.dbpedia.org/ns/core#> ;
	rdfs:label "Authorization Chain 7 property"@en;
    rdfs:comment "With the help of this property we can extend the reach dataid:authorizationScope over multiple instances of dataid:Dataset and dataid:Distribution."@en ;
    rdfs:range  prov:Entity ;
    owl:propertyChainAxiom (
    	dataid:authorizedFor
	    foaf:primaryTopic
	) .	
dataid:authorizationChain8
	a owl:ObjectProperty ;
	rdfs:subPropertyOf	dataid:authorizationScope ;
    rdfs:isDefinedBy <http://dataid.dbpedia.org/ns/core#> ;
	rdfs:label "Authorization Chain 8 property"@en;
    rdfs:comment "With the help of this property we can extend the reach dataid:authorizationScope over multiple instances of dataid:Dataset and dataid:Distribution."@en ;
    rdfs:range  prov:Entity ;
    owl:propertyChainAxiom (
	   dataid:authorizedFor
	   void:subset
	) .	
dataid:authorizationChain9
	a owl:ObjectProperty ;
	rdfs:subPropertyOf	dataid:authorizationScope ;
    rdfs:isDefinedBy <http://dataid.dbpedia.org/ns/core#> ;
	rdfs:label "Authorization Chain 9 property"@en;
    rdfs:comment "With the help of this property we can extend the reach dataid:authorizationScope over multiple instances of dataid:Dataset and dataid:Distribution."@en ;
    rdfs:range  prov:Entity ;
    owl:propertyChainAxiom (
	   dataid:authorizedFor
	   dcat:distribution
	) .
    
################### Individuals ####################

## Both ConceptSchemes are just examples in how to use AgentRoles and AuthorizedActions in the context of hierarchies.
## These Schemes are used to describe responsibilities of agents in the context of DataIDs and their Datasets.
## TopConcepts contain all actions (or roles) via the relations of skos:narrowerTransitive, skos:broaderTransitive.
dataid:AuthorizedActionScheme
	a owl:NamedIndividual, skos:ConceptScheme;
	skos:hasTopConcept dataid:AllResponsibilities, dataid:AllEntitlements ;
	rdfs:label "authorized action scheme"@en;
	rdfs:comment "Description of the AuthorizedAction hierarchy."@en .
	
dataid:AllResponsibilities
	a owl:NamedIndividual, dataid:ResponsibleAction ;
	rdfs:isDefinedBy <http://dataid.dbpedia.org/ns/core#> ;
	rdfs:comment "Encompasses all responsibilities (ResponsibleActions). The top concept of the AuthorizedActionScheme hierarchy."@en ;
	skos:prefLabel "all responsibilities"@en ;
	skos:topConceptOf dataid:AuthorizedActionScheme ;
	rdfs:label "all responsibilities"@en .
	
dataid:ResponseToContact
	a owl:NamedIndividual, dataid:ResponsibleAction ;
	rdfs:isDefinedBy <http://dataid.dbpedia.org/ns/core#> ;
	rdfs:comment "The responsibility (ResponsibleAction) to respond to contact attempts by external Agents. A contact point for the Entity."@en ;
	skos:prefLabel "response to contact attempt"@en ;
	skos:inScheme dataid:AuthorizedActionScheme ;
	skos:broader dataid:AllResponsibilities ;
	rdfs:label "response to contact attempt"@en .

dataid:ResponseToLifeCycleEvent
	a owl:NamedIndividual, dataid:ResponsibleAction ;
	rdfs:isDefinedBy <http://dataid.dbpedia.org/ns/core#> ;
	rdfs:comment "The responsibility (ResponsibleAction) to manage changes and react to bugs and issues that are reported concerning a Dataset."@en ;
	skos:prefLabel "response to life-cycle event"@en ;
	skos:inScheme dataid:AuthorizedActionScheme ;
	skos:broader dataid:AllResponsibilities ;
	rdfs:label "response to life-cycle event"@en .

dataid:PublishingDecision
	a owl:NamedIndividual, dataid:ResponsibleAction ;
	rdfs:isDefinedBy <http://dataid.dbpedia.org/ns/core#> ;
	rdfs:comment "The responsibility (ResponsibleAction) to decide if an Entity should be published."@en ;
	skos:prefLabel "publishing decision"@en ;
	skos:inScheme dataid:AuthorizedActionScheme ;
	skos:broader dataid:AllResponsibilities ;
	rdfs:label "publishing decision"@en .

dataid:UpdateDataId
	a owl:NamedIndividual, dataid:ResponsibleAction ;
	rdfs:isDefinedBy <http://dataid.dbpedia.org/ns/core#> ;
	rdfs:comment "The responsibility (ResponsibleAction) to update dataset metadata."@en ;
	skos:prefLabel "update DataId"@en ;
	skos:inScheme dataid:AuthorizedActionScheme ;
	skos:broader dataid:AllResponsibilities ;
	rdfs:label "update DataId"@en .

dataid:AgentSupervision
	a owl:NamedIndividual, dataid:ResponsibleAction ;
	rdfs:isDefinedBy <http://dataid.dbpedia.org/ns/core#> ;
	rdfs:comment "The responsibility (ResponsibleAction) to supervise other Agents."@en ;
	skos:prefLabel "agent supervision"@en ;
	skos:inScheme dataid:AuthorizedActionScheme ;
	skos:broader dataid:AllResponsibilities ;
	rdfs:label "agent supervision"@en .
	
dataid:AllEntitlements
	a owl:NamedIndividual, dataid:ResponsibleAction ;
	rdfs:isDefinedBy <http://dataid.dbpedia.org/ns/core#> ;
	rdfs:comment "Represents all entitlements (EntitledActions). The top concept of the AuthorizedActionScheme hierarchy."@en ;
	skos:prefLabel "all entitlements"@en ;
	skos:topConceptOf dataid:AuthorizedActionScheme ;
	rdfs:label "all entitlements"@en .

dataid:ReadDataId
	a owl:NamedIndividual, dataid:EntitledAction;
	rdfs:isDefinedBy <http://dataid.dbpedia.org/ns/core#> ;
	rdfs:comment "EntitledAction to read the DataID dataset metadata."@en ;
	skos:prefLabel "read DataID right"@en ;
	skos:inScheme dataid:AuthorizedActionScheme ;
	skos:broader dataid:AllEntitlements ;
	rdfs:label "read DataID right"@en .

dataid:ReadContent
	a owl:NamedIndividual, dataid:EntitledAction;
	rdfs:isDefinedBy <http://dataid.dbpedia.org/ns/core#> ;
	rdfs:comment "EntitledAction to read the content of an Entity."@en ;
	skos:prefLabel "read content right"@en ;
	skos:inScheme dataid:AuthorizedActionScheme ;
	skos:broader dataid:ModifyContent ;
	rdfs:label "read content right"@en .

dataid:ModifyContent
	a owl:NamedIndividual, dataid:EntitledAction;
	rdfs:isDefinedBy <http://dataid.dbpedia.org/ns/core#> ;
	rdfs:comment "EntitledAction to modify the content of an Entity."@en ;
	skos:prefLabel "modify content right"@en ;
	skos:inScheme dataid:AuthorizedActionScheme ;
	skos:broader dataid:DeleteContent ;
	rdfs:label "modify content right"@en .

dataid:DeleteContent
	a owl:NamedIndividual, dataid:EntitledAction;
	rdfs:isDefinedBy <http://dataid.dbpedia.org/ns/core#> ;
	rdfs:comment "EntitledAction to delete some content of an entity."@en ;
	skos:prefLabel "delete content right"@en ;
	skos:inScheme dataid:AuthorizedActionScheme ;
	skos:broader dataid:AllEntitlements ;
	rdfs:label "delete content right"@en .

dataid:ModifyAuthorizedAgents
	a owl:NamedIndividual, dataid:EntitledAction ;
	rdfs:comment "EntitledAction to modify which Agents are authorized on certain Entities."@en ;
	rdfs:isDefinedBy <http://dataid.dbpedia.org/ns/core#> ;
	skos:prefLabel "modify authorized agents"@en ;
	skos:inScheme dataid:AuthorizedActionScheme ;
	skos:broader dataid:AllEntitlements ;
	rdfs:label "modify authorized agents"@en .

dataid:ModifyAuthorization
	a owl:NamedIndividual, dataid:EntitledAction ;
	rdfs:comment "EntitledAction to modify an Authorization."@en ;
	rdfs:isDefinedBy <http://dataid.dbpedia.org/ns/core#> ;
	skos:prefLabel "modify authorization"@en ;
	skos:inScheme dataid:AuthorizedActionScheme ;
	skos:broader dataid:AllEntitlements ;
	rdfs:label "modify authorization"@en .

dataid:ModifyAgentRoles
	a owl:NamedIndividual, dataid:EntitledAction ;
	rdfs:comment "EntitledAction to modify the role of Agents on certain Entities."@en ;
	rdfs:isDefinedBy <http://dataid.dbpedia.org/ns/core#> ;
	skos:prefLabel "modify agent roles"@en ;
	skos:inScheme dataid:AuthorizedActionScheme ;
	skos:broader dataid:AllEntitlements ;
	rdfs:label "modify agent roles"@en .

dataid:AgentRoleScheme
	a owl:NamedIndividual, skos:ConceptScheme ;
	skos:hasTopConcept dataid:Creator ;
	rdfs:label "agent role scheme"@en;
	rdfs:comment "The AgentRole scheme (hierarchy) provided by DataID core, depicting Roles commonly used in the context of a file or document management system. This scheme should be replaced in other use cases."@en .

dataid:Creator
	a owl:NamedIndividual, dataid:AgentRole;
	rdfs:isDefinedBy <http://dataid.dbpedia.org/ns/core#> ;
	dataid:allowsFor dataid:AllResponsibilities, dataid:AllEntitlements ;
    rdfs:comment "Creator of the resource. An AgentRole that is credited with the main part in the initial creation of the resource."@en ;
    skos:prefLabel "creator"@en ;
	skos:topConceptOf dataid:AgentRoleScheme ;
	rdfs:label "creator"@en .

dataid:Publisher
	a owl:NamedIndividual, dataid:AgentRole;
	rdfs:isDefinedBy <http://dataid.dbpedia.org/ns/core#> ;
	dataid:allowsFor dataid:ReadDataId;
	dataid:allowsFor dataid:UpdateDataId;
	dataid:allowsFor dataid:ModifyContent;
	dataid:allowsFor dataid:DeleteContent;
	dataid:allowsFor dataid:ReadContent;
	dataid:allowsFor dataid:ModifyAuthorizedAgents;
	dataid:allowsFor dataid:ResponseToLifeCycleEvent;
	dataid:allowsFor dataid:ResponseToContact;
	dataid:allowsFor dataid:AgentSupervision;
	dataid:allowsFor dataid:PublishingDecision;
	dataid:allowsFor dataid:ModifyAuthorization;
    rdfs:comment "Publisher of the Dataset. An Agent that makes the Dataset accessible online on a server or repository without necessarily being involved in its creation."@en ;
    skos:prefLabel "publisher"@en ;
	skos:inScheme dataid:AgentRoleScheme ;
	skos:broader dataid:Creator ;
	rdfs:label "publisher"@en .

dataid:Maintainer
	a owl:NamedIndividual, dataid:AgentRole;
	rdfs:isDefinedBy <http://dataid.dbpedia.org/ns/core#> ;
	dataid:allowsFor dataid:ReadDataId;
	dataid:allowsFor dataid:UpdateDataId;
	dataid:allowsFor dataid:ModifyContent;
	dataid:allowsFor dataid:DeleteContent;
	dataid:allowsFor dataid:ReadContent;
	dataid:allowsFor dataid:ModifyAuthorizedAgents;
	dataid:allowsFor dataid:ResponseToLifeCycleEvent;
	dataid:allowsFor dataid:ResponseToContact;
    rdfs:comment "Maintainer of the Dataset. An Agent that ensures the technical correctness, accessibility and up-to-dateness of a Dataset."@en ;
    skos:prefLabel "maintainer"@en ;
	skos:inScheme dataid:AgentRoleScheme ;
	skos:broader dataid:Creator ;
	rdfs:label "maintainer"@en .

dataid:Contributor
	a owl:NamedIndividual, dataid:AgentRole;
	rdfs:isDefinedBy <http://dataid.dbpedia.org/ns/core#> ;
	dataid:allowsFor dataid:ReadDataId;
	dataid:allowsFor dataid:ReadContent;
	rdfs:comment "Contributor to the resource. An Agent that was involved in creating or maintaining the resource but does not have the main part in this activity."@en ;
	skos:prefLabel "contributor"@en ;
	skos:inScheme dataid:AgentRoleScheme ;
	skos:broader dataid:Publisher ;
	rdfs:label "contributor"@en .

dataid:Contact
	a owl:NamedIndividual, dataid:AgentRole;
	rdfs:isDefinedBy <http://dataid.dbpedia.org/ns/core#> ;
	dataid:allowsFor dataid:ReadDataId;
	dataid:allowsFor dataid:ModifyContent;
	dataid:allowsFor dataid:ReadContent;
	dataid:allowsFor dataid:ResponseToContact;
    rdfs:comment "Contact agent. An Agent that can be contacted for general requests about the resource."@en ;
    skos:prefLabel "contact"@en ;
	skos:inScheme dataid:AgentRoleScheme ;
	skos:broader dataid:Publisher, dataid:Maintainer ;
	rdfs:label "contact"@en .

dataid:Guest
	a owl:NamedIndividual, dataid:AgentRole;
	dataid:allowsFor dataid:ReadDataId;
	dataid:allowsFor dataid:ReadContent;
	rdfs:isDefinedBy <http://dataid.dbpedia.org/ns/core#> ;
    rdfs:comment "A visitor or anonymous Agent has only read rights on public documents"@en ;
    skos:prefLabel "guest"@en ;
	skos:inScheme dataid:AgentRoleScheme ;
	skos:broader dataid:Contributor ;
	rdfs:label "guest"@en .

#defining the generic Agent for any Agent not specifically defined
dataid:GuestAgent
    a owl:NamedIndividual, dataid:Agent;
    rdfs:isDefinedBy <http://dataid.dbpedia.org/ns/core#> ;
    rdfs:comment "Use this Agent as a stand in for any Agent not specifically defined in a domain, granting public access to an Entity."@en ;
    rdfs:label "guest agent"@en ;
    foaf:mbox 		<mailto:address@alibi.com> ;
    foaf:homepage  <http://dataid.dbpedia.org>;
    foaf:name   "Guest Agent".
    
dataid:GuestAuthorization
	a owl:NamedIndividual, dataid:Authorization ;
    rdfs:isDefinedBy <http://dataid.dbpedia.org/ns/core#> ;
	dataid:isInheritable true ;
	dataid:authorizedAgent dataid:GuestAgent ;
	dataid:authorityAgentRole dataid:Guest ;
	rdfs:label "guest authority"@en ;
	rdfs:comment "This Authorization can be used to point out that the content of an entity is public and can be read by anyone (see also dataid:Guest)."@en .
	
# DatasetRelationRoles	
dataid:GenericRelation
	a owl:NamedIndividual, dataid:DatasetRelationRole;
    rdfs:isDefinedBy <http://dataid.dbpedia.org/ns/core#> ;
    rdfs:label "Generic Relation"@en ;
    rdfs:comment "This role specifies a dataid:DatasetRelationship between two datasets which have a relation of a unknown quality."@en .
    
dataid:DerivatRole
	a owl:NamedIndividual, dataid:DatasetRelationRole;
    rdfs:isDefinedBy <http://dataid.dbpedia.org/ns/core#> ;
    rdfs:label "Derivat Role"@en ;
    rdfs:comment "This role specifies a dataid:DatasetRelationship where one dataset points out a second dataset, which is a derivat of the first."@en .
	
dataid:SourceRole
	a owl:NamedIndividual, dataid:DatasetRelationRole;
    rdfs:isDefinedBy <http://dataid.dbpedia.org/ns/core#> ;
    rdfs:label "Source Role"@en ;
    rdfs:comment "This role specifies a dataid:DatasetRelationship where the origin dataset is created by transforming/collecting data from the target dataset."@en .

dataid:CopyRole
	a owl:NamedIndividual, dataid:DatasetRelationRole;
    rdfs:isDefinedBy <http://dataid.dbpedia.org/ns/core#> ;
    rdfs:label "Copy Role"@en ;
    rdfs:comment "This role specifies a dataid:DatasetRelationship where the origin dataset is an exact copy of the target dataset (e.g. when republished under a different domain)."@en .
    
dataid:SimilarityRole
	a owl:NamedIndividual, dataid:DatasetRelationRole;
    rdfs:isDefinedBy <http://dataid.dbpedia.org/ns/core#> ;
    rdfs:label "Similarity Role"@en ;
    rdfs:comment "This role specifies a dataid:DatasetRelationship where the origin dataset has a significant similarity to the target dataset (without any assertion as to dimension of similarity)."@en .